modifs

TP6/practica6.v
@@ -1,3 +1,5 @@
+Extraction Language Haskell.
+
 Section Ejercicio1.
 
 (* 1.1 *)
@@ -14,8 +16,71 @@ Qed.
 End Ejercicio1.
 
 (* 1.2 *)
-Extraction Language Haskell.
 Extraction "predecesor" predspec.
+
+Section Ejercicio2.
+
+Inductive bintree (X:Set) :=
+  Empty : bintree X
+  | Branch : X -> bintree X -> bintree X -> bintree X.
+
+Inductive mirror (X:Set) : bintree X -> bintree X -> Prop :=
+  mirror_empty : mirror X (Empty X) (Empty X)
+  | mirror_branch : forall (t11 t12 t21 t22 : bintree X) (x1 x2 : X),
+    mirror X t11 t22 -> mirror X t12 t21 ->
+      x1 = x2 -> mirror X (Branch X x1 t11 t12) (Branch X x2 t21 t22).
+
+(* 2.1 *)
+Lemma MirrorC: forall (A:Set) (t:bintree A),
+{t':bintree A|(mirror A t t')}.
+Proof.
+  intros.
+  induction t.
+    exists (Empty A).
+    constructor.
+
+    destruct IHt1.
+    destruct IHt2.
+    exists (Branch A x x1 x0).
+    constructor; trivial.
+Qed.
+
+(* 2.2 *)
+Fixpoint inverse (X : Set) (b : bintree X) : bintree X :=
+  match b with
+    Empty => Empty X
+    | (Branch e l r) => Branch X e (inverse X r) (inverse X l)
+  end.
+
+Hint Constructors mirror.
+
+Lemma MirrorC2: forall (A:Set) (t:bintree A),
+{ t' : bintree A | (mirror A t t') /\ t' = inverse A t}.
+Proof.
+  intros.
+  induction t.
+    simpl.
+    exists (Empty A).
+    split; trivial.
+
+    simpl.
+    destruct IHt1.
+    destruct IHt2.
+    exists (Branch A x (inverse A t2) (inverse A t1)).
+    split;
+    [ destruct a;
+      destruct a0;
+      constructor;
+      [ rewrite H0 in H
+      | rewrite H2 in H1
+      | ]
+    | ]; trivial.
+Qed.
+
+End Ejercicio2.
+
+(* 2.3 *)
+Extraction "mirror_function" MirrorC2.
 
 Section Ejercicio3.
 
@@ -23,18 +88,20 @@ Section Ejercicio3.
 Definition Value := bool.
 
 Inductive BoolExpr : Set :=
-| bbool : bool -> BoolExpr
-| or : BoolExpr -> BoolExpr -> BoolExpr
-| bnot : BoolExpr -> BoolExpr.
+  | bbool : bool -> BoolExpr
+  | or : BoolExpr -> BoolExpr -> BoolExpr
+  | bnot : BoolExpr -> BoolExpr.
 
 Inductive BEval : BoolExpr -> Value -> Prop :=
-| ebool : forall b : bool, BEval (bbool b) (b:Value)
-| eorl : forall e1 e2 : BoolExpr, BEval e1 true -> BEval (or e1 e2) true
-| eorr : forall e1 e2 : BoolExpr, BEval e2 true -> BEval (or e1 e2) true
-| eorrl : forall e1 e2 : BoolExpr,
-BEval e1 false -> BEval e2 false -> BEval (or e1 e2) false
-| enott : forall e : BoolExpr, BEval e true -> BEval (bnot e) false
-| enotf : forall e : BoolExpr, BEval e false -> BEval (bnot e) true.
+  | ebool : forall b : bool, BEval (bbool b) (b:Value)
+  | eorl : forall e1 e2 : BoolExpr,
+    BEval e1 true -> BEval (or e1 e2) true
+  | eorr : forall e1 e2 : BoolExpr,
+    BEval e2 true -> BEval (or e1 e2) true
+  | eorrl : forall e1 e2 : BoolExpr,
+    BEval e1 false -> BEval e2 false -> BEval (or e1 e2) false
+  | enott : forall e : BoolExpr, BEval e true -> BEval (bnot e) false
+  | enotf : forall e : BoolExpr, BEval e false -> BEval (bnot e) true.
 
 Fixpoint beval (e : BoolExpr) : Value :=
   match e with
@@ -58,4 +125,64 @@ Fixpoint sbeval (e : BoolExpr) : Value :=
     | bnot e1 => if sbeval e1 then false else true
   end.
 
+
+
 End Ejercicio3.
+
+Section Ejercicio4.
+
+Variable A:Set.
+
+Inductive list : Set :=
+  | nil : list
+  | cons : A -> list -> list.
+
+Fixpoint append (l1 l2 : list) {struct l1} : list :=
+  match l1 with
+    | nil => l2
+    | cons a l => cons a (append l l2)
+  end.
+
+Inductive perm : list -> list ->Prop:=
+  | perm_refl: forall l, perm l l
+  | perm_cons: forall a l0 l1, perm l0 l1-> perm (cons a l0)(cons a l1)
+  | perm_app: forall a l, perm (cons a l) (append l (cons a nil))
+  | perm_trans: forall l1 l2 l3, perm l1 l2 -> perm l2 l3 -> perm l1 l3.
+
+Hint Constructors perm.
+
+(* 4.1 *)
+Fixpoint reverse (l : list) : list :=
+  match l with
+    | nil => nil
+    | cons x xs => append (reverse xs) (cons x nil)
+  end.
+
+(* 4.2 *)
+Lemma Ej6_4: forall l: list, {l2: list | perm l l2}.
+Proof.
+  induction l.
+    exists nil.
+    constructor.
+
+    destruct IHl.
+    exists (cons a x).
+    constructor.
+    trivial.
+Qed.
+
+Lemma Ej6_4_2: forall l: list,
+  {l2: list | l2 = reverse l -> perm l l2}.
+Proof.
+  induction l.
+    exists nil.
+    constructor.
+
+    simpl.
+    destruct IHl.
+    exists (append x (cons a nil)).
+    intros.
+    
+Qed.
+
+End Ejercicio4.
